---
weight: 2
---

{{< tabs "32eed228" >}}

{{< tab "Standard view" >}}

<style type="text/css">
#T_standard_3545fcb7f817fb6a th.col_heading {
  text-align: left;
  font-size: 1em;
}
#T_standard_3545fcb7f817fb6a td {
  text-align: left;
  font-size: 1em;
  padding: 1.5em;
}
</style>
<table id="T_standard_3545fcb7f817fb6a">
  <thead>
  </thead>
  <tbody>
    <tr>
      <td id="T_standard_3545fcb7f817fb6a_row0_col0" class="data row0 col0" >Logistic equation option 1: $\frac{dP}{dt} = kP(N-P)$ <br><br></td>
    </tr>
    <tr>
      <td id="T_standard_3545fcb7f817fb6a_row1_col0" class="data row1 col0" >Logistic equation option 2:$\frac{dP}{dt} = kP(1-\frac{P}{N})$</td>
    </tr>
    <tr>
      <td id="T_standard_3545fcb7f817fb6a_row2_col0" class="data row2 col0" >$y=\sin^{-1}f(x) \,\,\,\,\,\,\,\,\,\,\,\,\,\,\,\,\,\,\,\,\,\,\,\,\,\,\,\,\,\,\,\,\,\,\,\,\,   \dfrac{dy}{dx} = \dfrac{f'(x)} {\sqrt {1 - (f(x))^2} }$ <br></td>
    </tr>
    <tr>
      <td id="T_standard_3545fcb7f817fb6a_row3_col0" class="data row3 col0" >$ y = \sin^{-1} \dfrac{f(x)}{a}  \,\,\,\,\,\,\,\,\,\,\,\,\,\,\,\,\,\,\,\,\,\,\,\,\,\,\,\,\,\,\,\,\,\,\,   \dfrac{dy}{dx} = \dfrac{f'(x)}{\sqrt{a^2 - (f(x))^2}} $ <br></td>
    </tr>
    <tr>
      <td id="T_standard_3545fcb7f817fb6a_row4_col0" class="data row4 col0" >$y=\cos^{-1}f(x) \,\,\,\,\,\,\,\,\,\,\,\,\,\,\,\,\,\,\,\,\,\,\,\,\,\,\,\,\,\,\,\,\,\,\,\,\,   \dfrac{dy}{dx} = - \dfrac{f'(x)} {\sqrt {1 - (f(x))^2} }$ <br></td>
    </tr>
    <tr>
      <td id="T_standard_3545fcb7f817fb6a_row5_col0" class="data row5 col0" >$y=\cos^{-1} \dfrac{f(x)}{a} \,\,\,\,\,\,\,\,\,\,\,\,\,\,\,\,\,\,\,\,\,\,\,\,\,\,\,\,\,\,\,\,\,\,\,   \dfrac{dy}{dx} = - \dfrac{f'(x)} {\sqrt {a^2 - (f(x))^2} }$ <br></td>
    </tr>
    <tr>
      <td id="T_standard_3545fcb7f817fb6a_row6_col0" class="data row6 col0" >$y=\tan^{-1}f(x) \,\,\,\,\,\,\,\,\,\,\,\,\,\,\,\,\,\,\,\,\,\,\,\,\,\,\,\,\,\,\,\,\,\,\,\,\,   \dfrac{dy}{dx} = \dfrac{f'(x)} {1 + (f(x))^2}$ <br></td>
    </tr>
    <tr>
      <td id="T_standard_3545fcb7f817fb6a_row7_col0" class="data row7 col0" >$y=\tan^{-1}\dfrac{f(x)}{a} \,\,\,\,\,\,\,\,\,\,\,\,\,\,\,\,\,\,\,\,\,\,\,\,\,\,\,\,\,\,\,\,\,\,\,   \dfrac{dy}{dx} =  \dfrac{1}{a} \tan^{-1} \dfrac{f(x)}{a} $ <br></td>
    </tr>
    <tr>
      <td id="T_standard_3545fcb7f817fb6a_row8_col0" class="data row8 col0" >$ \text{Function and its inverse}  \,\,\,\,\,\,\,\,\,\,\,\,\,   \dfrac{dy}{dx} \times \dfrac{dx}{dy} = 1, \text{  or  } \dfrac{dy}{dx} = \dfrac{1}{\dfrac{dx}{dy}} $ <br></td>
    </tr>
  </tbody>
</table>
{{< /tab >}}

{{< tab "Formula sheet" >}}

Items on formula sheet are highlighted 
<br>
<style type="text/css">
#T_formula_sheet_31f995a0f4499e1d th.col_heading {
  text-align: left;
  font-size: 1em;
}
#T_formula_sheet_31f995a0f4499e1d td {
  text-align: left;
  font-size: 1em;
  padding: 1.5em;
}
#T_formula_sheet_31f995a0f4499e1d_row0_col0, #T_formula_sheet_31f995a0f4499e1d_row1_col0, #T_formula_sheet_31f995a0f4499e1d_row3_col0, #T_formula_sheet_31f995a0f4499e1d_row5_col0, #T_formula_sheet_31f995a0f4499e1d_row7_col0, #T_formula_sheet_31f995a0f4499e1d_row8_col0 {
  background-color: rgba(0,0,0,0);
}
#T_formula_sheet_31f995a0f4499e1d_row2_col0, #T_formula_sheet_31f995a0f4499e1d_row4_col0, #T_formula_sheet_31f995a0f4499e1d_row6_col0 {
  background-color: rgba(255,194,10, 0.2);
}
</style>
<table id="T_formula_sheet_31f995a0f4499e1d">
  <thead>
  </thead>
  <tbody>
    <tr>
      <td id="T_formula_sheet_31f995a0f4499e1d_row0_col0" class="data row0 col0" >Logistic equation option 1: $\frac{dP}{dt} = kP(N-P)$ <br><br></td>
    </tr>
    <tr>
      <td id="T_formula_sheet_31f995a0f4499e1d_row1_col0" class="data row1 col0" >Logistic equation option 2:$\frac{dP}{dt} = kP(1-\frac{P}{N})$</td>
    </tr>
    <tr>
      <td id="T_formula_sheet_31f995a0f4499e1d_row2_col0" class="data row2 col0" >$y=\sin^{-1}f(x) \,\,\,\,\,\,\,\,\,\,\,\,\,\,\,\,\,\,\,\,\,\,\,\,\,\,\,\,\,\,\,\,\,\,\,\,\,   \dfrac{dy}{dx} = \dfrac{f'(x)} {\sqrt {1 - (f(x))^2} }$ <br></td>
    </tr>
    <tr>
      <td id="T_formula_sheet_31f995a0f4499e1d_row3_col0" class="data row3 col0" >$ y = \sin^{-1} \dfrac{f(x)}{a}  \,\,\,\,\,\,\,\,\,\,\,\,\,\,\,\,\,\,\,\,\,\,\,\,\,\,\,\,\,\,\,\,\,\,\,   \dfrac{dy}{dx} = \dfrac{f'(x)}{\sqrt{a^2 - (f(x))^2}} $ <br></td>
    </tr>
    <tr>
      <td id="T_formula_sheet_31f995a0f4499e1d_row4_col0" class="data row4 col0" >$y=\cos^{-1}f(x) \,\,\,\,\,\,\,\,\,\,\,\,\,\,\,\,\,\,\,\,\,\,\,\,\,\,\,\,\,\,\,\,\,\,\,\,\,   \dfrac{dy}{dx} = - \dfrac{f'(x)} {\sqrt {1 - (f(x))^2} }$ <br></td>
    </tr>
    <tr>
      <td id="T_formula_sheet_31f995a0f4499e1d_row5_col0" class="data row5 col0" >$y=\cos^{-1} \dfrac{f(x)}{a} \,\,\,\,\,\,\,\,\,\,\,\,\,\,\,\,\,\,\,\,\,\,\,\,\,\,\,\,\,\,\,\,\,\,\,   \dfrac{dy}{dx} = - \dfrac{f'(x)} {\sqrt {a^2 - (f(x))^2} }$ <br></td>
    </tr>
    <tr>
      <td id="T_formula_sheet_31f995a0f4499e1d_row6_col0" class="data row6 col0" >$y=\tan^{-1}f(x) \,\,\,\,\,\,\,\,\,\,\,\,\,\,\,\,\,\,\,\,\,\,\,\,\,\,\,\,\,\,\,\,\,\,\,\,\,   \dfrac{dy}{dx} = \dfrac{f'(x)} {1 + (f(x))^2}$ <br></td>
    </tr>
    <tr>
      <td id="T_formula_sheet_31f995a0f4499e1d_row7_col0" class="data row7 col0" >$y=\tan^{-1}\dfrac{f(x)}{a} \,\,\,\,\,\,\,\,\,\,\,\,\,\,\,\,\,\,\,\,\,\,\,\,\,\,\,\,\,\,\,\,\,\,\,   \dfrac{dy}{dx} =  \dfrac{1}{a} \tan^{-1} \dfrac{f(x)}{a} $ <br></td>
    </tr>
    <tr>
      <td id="T_formula_sheet_31f995a0f4499e1d_row8_col0" class="data row8 col0" >$ \text{Function and its inverse}  \,\,\,\,\,\,\,\,\,\,\,\,\,   \dfrac{dy}{dx} \times \dfrac{dx}{dy} = 1, \text{  or  } \dfrac{dy}{dx} = \dfrac{1}{\dfrac{dx}{dy}} $ <br></td>
    </tr>
  </tbody>
</table>
{{< /tab >}}

{{< tab "Proofs required" >}}

Items where proofs required are highlighted 
<br>
<style type="text/css">
#T_proof_required_af82adb4400bd3be th.col_heading {
  text-align: left;
  font-size: 1em;
}
#T_proof_required_af82adb4400bd3be td {
  text-align: left;
  font-size: 1em;
  padding: 1.5em;
}
#T_proof_required_af82adb4400bd3be_row0_col0, #T_proof_required_af82adb4400bd3be_row1_col0, #T_proof_required_af82adb4400bd3be_row8_col0 {
  background-color: rgba(0,0,0,0);
}
#T_proof_required_af82adb4400bd3be_row2_col0, #T_proof_required_af82adb4400bd3be_row3_col0, #T_proof_required_af82adb4400bd3be_row4_col0, #T_proof_required_af82adb4400bd3be_row5_col0, #T_proof_required_af82adb4400bd3be_row6_col0, #T_proof_required_af82adb4400bd3be_row7_col0 {
  background-color: rgba(0,150,200, 0.2);
}
</style>
<table id="T_proof_required_af82adb4400bd3be">
  <thead>
  </thead>
  <tbody>
    <tr>
      <td id="T_proof_required_af82adb4400bd3be_row0_col0" class="data row0 col0" >Logistic equation option 1: $\frac{dP}{dt} = kP(N-P)$ <br><br></td>
    </tr>
    <tr>
      <td id="T_proof_required_af82adb4400bd3be_row1_col0" class="data row1 col0" >Logistic equation option 2:$\frac{dP}{dt} = kP(1-\frac{P}{N})$</td>
    </tr>
    <tr>
      <td id="T_proof_required_af82adb4400bd3be_row2_col0" class="data row2 col0" >$y=\sin^{-1}f(x) \,\,\,\,\,\,\,\,\,\,\,\,\,\,\,\,\,\,\,\,\,\,\,\,\,\,\,\,\,\,\,\,\,\,\,\,\,   \dfrac{dy}{dx} = \dfrac{f'(x)} {\sqrt {1 - (f(x))^2} }$ <br></td>
    </tr>
    <tr>
      <td id="T_proof_required_af82adb4400bd3be_row3_col0" class="data row3 col0" >$ y = \sin^{-1} \dfrac{f(x)}{a}  \,\,\,\,\,\,\,\,\,\,\,\,\,\,\,\,\,\,\,\,\,\,\,\,\,\,\,\,\,\,\,\,\,\,\,   \dfrac{dy}{dx} = \dfrac{f'(x)}{\sqrt{a^2 - (f(x))^2}} $ <br></td>
    </tr>
    <tr>
      <td id="T_proof_required_af82adb4400bd3be_row4_col0" class="data row4 col0" >$y=\cos^{-1}f(x) \,\,\,\,\,\,\,\,\,\,\,\,\,\,\,\,\,\,\,\,\,\,\,\,\,\,\,\,\,\,\,\,\,\,\,\,\,   \dfrac{dy}{dx} = - \dfrac{f'(x)} {\sqrt {1 - (f(x))^2} }$ <br></td>
    </tr>
    <tr>
      <td id="T_proof_required_af82adb4400bd3be_row5_col0" class="data row5 col0" >$y=\cos^{-1} \dfrac{f(x)}{a} \,\,\,\,\,\,\,\,\,\,\,\,\,\,\,\,\,\,\,\,\,\,\,\,\,\,\,\,\,\,\,\,\,\,\,   \dfrac{dy}{dx} = - \dfrac{f'(x)} {\sqrt {a^2 - (f(x))^2} }$ <br></td>
    </tr>
    <tr>
      <td id="T_proof_required_af82adb4400bd3be_row6_col0" class="data row6 col0" >$y=\tan^{-1}f(x) \,\,\,\,\,\,\,\,\,\,\,\,\,\,\,\,\,\,\,\,\,\,\,\,\,\,\,\,\,\,\,\,\,\,\,\,\,   \dfrac{dy}{dx} = \dfrac{f'(x)} {1 + (f(x))^2}$ <br></td>
    </tr>
    <tr>
      <td id="T_proof_required_af82adb4400bd3be_row7_col0" class="data row7 col0" >$y=\tan^{-1}\dfrac{f(x)}{a} \,\,\,\,\,\,\,\,\,\,\,\,\,\,\,\,\,\,\,\,\,\,\,\,\,\,\,\,\,\,\,\,\,\,\,   \dfrac{dy}{dx} =  \dfrac{1}{a} \tan^{-1} \dfrac{f(x)}{a} $ <br></td>
    </tr>
    <tr>
      <td id="T_proof_required_af82adb4400bd3be_row8_col0" class="data row8 col0" >$ \text{Function and its inverse}  \,\,\,\,\,\,\,\,\,\,\,\,\,   \dfrac{dy}{dx} \times \dfrac{dx}{dy} = 1, \text{  or  } \dfrac{dy}{dx} = \dfrac{1}{\dfrac{dx}{dy}} $ <br></td>
    </tr>
  </tbody>
</table>
{{< /tab >}}
{{< /tabs >}}