---
weight: 8
---

{{< tabs "9d75f33f" >}}

{{< tab "Standard view" >}}

<style type="text/css">
#T_standard_cc50b2d6a18fcab8 th.col_heading {
  text-align: left;
  font-size: 1em;
}
#T_standard_cc50b2d6a18fcab8 td {
  text-align: left;
  font-size: 1em;
  padding: 1.5em;
}
</style>
<table id="T_standard_cc50b2d6a18fcab8">
  <thead>
  </thead>
  <tbody>
    <tr>
      <td id="T_standard_cc50b2d6a18fcab8_row0_col0" class="data row0 col0" >$ {\Large\int} f'(x)[f(x)]^n dx = \dfrac{1}{n+1}[f(x)]^{n+1} + c $
$ \text{ where } n \neq -1 $</td>
    </tr>
    <tr>
      <td id="T_standard_cc50b2d6a18fcab8_row1_col0" class="data row1 col0" >$ {\Large\int} u \dfrac{dv}{dx} dx=uv-{\Large\int}v \dfrac {du}{dx}dx$</td>
    </tr>
    <tr>
      <td id="T_standard_cc50b2d6a18fcab8_row2_col0" class="data row2 col0" >$ {\Large\int_{a}^{b}} f(x) dx \approx \dfrac{b-a} {2n} {\Large\{} f(a) + f(b) + 2 {\Large[} f(x_1)+...+f(x_{n-1}){\Large ]} {\Large\}}$
$ \text { where } a=x_0 \text{ and } b=x_n $</td>
    </tr>
    <tr>
      <td id="T_standard_cc50b2d6a18fcab8_row3_col0" class="data row3 col0" >Volumes formed by rotation about the x-axis = $V=\pi \int_a^b y^2 dx$</td>
    </tr>
    <tr>
      <td id="T_standard_cc50b2d6a18fcab8_row4_col0" class="data row4 col0" >Volumes formed by rotation about the y-axis = $V=\pi \int_a^b x^2 dy$</td>
    </tr>
    <tr>
      <td id="T_standard_cc50b2d6a18fcab8_row5_col0" class="data row5 col0" >$ {\Large\int} f'(x)\cos f(x)dx = \sin f(x) + c$</td>
    </tr>
    <tr>
      <td id="T_standard_cc50b2d6a18fcab8_row6_col0" class="data row6 col0" >$ {\Large\int} f'(x)\sin f(x)dx = -\cos f(x) + c$</td>
    </tr>
    <tr>
      <td id="T_standard_cc50b2d6a18fcab8_row7_col0" class="data row7 col0" >$ {\Large\int} f'(x)\sec^2 f(x)dx = \tan f(x) + c$</td>
    </tr>
    <tr>
      <td id="T_standard_cc50b2d6a18fcab8_row8_col0" class="data row8 col0" >$ {\Large\int} f'(x)e^{f(x)}dx = e^{f(x)} + c$</td>
    </tr>
    <tr>
      <td id="T_standard_cc50b2d6a18fcab8_row9_col0" class="data row9 col0" >$ {\Large\int} \dfrac{f'(x)}{f(x)}dx = \ln|f(x)| + c$</td>
    </tr>
    <tr>
      <td id="T_standard_cc50b2d6a18fcab8_row10_col0" class="data row10 col0" >$ {\Large\int} f'(x)a^{f(x)}dx = \dfrac{a^f(x)}{\ln  a} +c$</td>
    </tr>
    <tr>
      <td id="T_standard_cc50b2d6a18fcab8_row11_col0" class="data row11 col0" >$ {\Large\int} \dfrac{f'(x)}{(\ln a) f(x)} = \log_{a} |f(x)|  + c$</td>
    </tr>
    <tr>
      <td id="T_standard_cc50b2d6a18fcab8_row12_col0" class="data row12 col0" >$ {\Large\int}_b^a f(x)dx = F(b)-F(a) \text{, where F(x) is the anti-derivative of f(x)}$</td>
    </tr>
    <tr>
      <td id="T_standard_cc50b2d6a18fcab8_row13_col0" class="data row13 col0" >$F'(x) = \dfrac{d}{dx} {\Large\int}_a^x f(t)dt = f(x) \text{ (the Fundamental Therom of Calculus)}$</td>
    </tr>
    <tr>
      <td id="T_standard_cc50b2d6a18fcab8_row14_col0" class="data row14 col0" >$ {\Large\int} \dfrac{f'(x)} {\sqrt {1 - (f(x))^2} } dx = \sin^{-1} f(x) + c$</td>
    </tr>
    <tr>
      <td id="T_standard_cc50b2d6a18fcab8_row15_col0" class="data row15 col0" >$ {\Large\int} \dfrac{f'(x)} {\sqrt {a^2 - (f(x))^2} } dx = \sin^{-1} \dfrac{f(x)}{a} + c$</td>
    </tr>
    <tr>
      <td id="T_standard_cc50b2d6a18fcab8_row16_col0" class="data row16 col0" >$ {\Large\int} - \dfrac{f'(x)} {\sqrt {1 - (f(x))^2} }  = \cos^{-1}f(x) + c \text{ or } -\sin^{-1}f(x) +c$
$ \text{Note the constant c will have different values with these two options} $</td>
    </tr>
    <tr>
      <td id="T_standard_cc50b2d6a18fcab8_row17_col0" class="data row17 col0" >$ {\Large\int} - \dfrac{f'(x)} {\sqrt {a^2 - (f(x))^2} }  = \cos^{-1}\dfrac{f(x)}{a} + c \text{ or } -\sin^{-1}\dfrac{f(x)}{a} +c$
$ \text{Note the constant c will have different values with these two options} $</td>
    </tr>
    <tr>
      <td id="T_standard_cc50b2d6a18fcab8_row18_col0" class="data row18 col0" >$ {\Large\int} \dfrac{f'(x)} {1 + (f(x))^2} dx = \ \tan^{-1} f(x) + c$</td>
    </tr>
    <tr>
      <td id="T_standard_cc50b2d6a18fcab8_row19_col0" class="data row19 col0" >$ {\Large\int} \dfrac{f'(x)} {a^2 + (f(x))^2} dx = \dfrac{1}{a} \tan^{-1} \dfrac{f(x)}{a} + c$</td>
    </tr>
  </tbody>
</table>
{{< /tab >}}

{{< tab "Formula sheet" >}}

Items on formula sheet are highlighted 
<br>
<style type="text/css">
#T_formula_sheet_ab3cf35d4f5e6964 th.col_heading {
  text-align: left;
  font-size: 1em;
}
#T_formula_sheet_ab3cf35d4f5e6964 td {
  text-align: left;
  font-size: 1em;
  padding: 1.5em;
}
#T_formula_sheet_ab3cf35d4f5e6964_row0_col0, #T_formula_sheet_ab3cf35d4f5e6964_row1_col0, #T_formula_sheet_ab3cf35d4f5e6964_row2_col0, #T_formula_sheet_ab3cf35d4f5e6964_row5_col0, #T_formula_sheet_ab3cf35d4f5e6964_row6_col0, #T_formula_sheet_ab3cf35d4f5e6964_row7_col0, #T_formula_sheet_ab3cf35d4f5e6964_row8_col0, #T_formula_sheet_ab3cf35d4f5e6964_row9_col0, #T_formula_sheet_ab3cf35d4f5e6964_row10_col0, #T_formula_sheet_ab3cf35d4f5e6964_row15_col0, #T_formula_sheet_ab3cf35d4f5e6964_row19_col0 {
  background-color: rgba(255,194,10, 0.2);
}
#T_formula_sheet_ab3cf35d4f5e6964_row3_col0, #T_formula_sheet_ab3cf35d4f5e6964_row4_col0, #T_formula_sheet_ab3cf35d4f5e6964_row11_col0, #T_formula_sheet_ab3cf35d4f5e6964_row12_col0, #T_formula_sheet_ab3cf35d4f5e6964_row13_col0, #T_formula_sheet_ab3cf35d4f5e6964_row14_col0, #T_formula_sheet_ab3cf35d4f5e6964_row16_col0, #T_formula_sheet_ab3cf35d4f5e6964_row17_col0, #T_formula_sheet_ab3cf35d4f5e6964_row18_col0 {
  background-color: rgba(0,0,0,0);
}
</style>
<table id="T_formula_sheet_ab3cf35d4f5e6964">
  <thead>
  </thead>
  <tbody>
    <tr>
      <td id="T_formula_sheet_ab3cf35d4f5e6964_row0_col0" class="data row0 col0" >$ {\Large\int} f'(x)[f(x)]^n dx = \dfrac{1}{n+1}[f(x)]^{n+1} + c $
$ \text{ where } n \neq -1 $</td>
    </tr>
    <tr>
      <td id="T_formula_sheet_ab3cf35d4f5e6964_row1_col0" class="data row1 col0" >$ {\Large\int} u \dfrac{dv}{dx} dx=uv-{\Large\int}v \dfrac {du}{dx}dx$</td>
    </tr>
    <tr>
      <td id="T_formula_sheet_ab3cf35d4f5e6964_row2_col0" class="data row2 col0" >$ {\Large\int_{a}^{b}} f(x) dx \approx \dfrac{b-a} {2n} {\Large\{} f(a) + f(b) + 2 {\Large[} f(x_1)+...+f(x_{n-1}){\Large ]} {\Large\}}$
$ \text { where } a=x_0 \text{ and } b=x_n $</td>
    </tr>
    <tr>
      <td id="T_formula_sheet_ab3cf35d4f5e6964_row3_col0" class="data row3 col0" >Volumes formed by rotation about the x-axis = $V=\pi \int_a^b y^2 dx$</td>
    </tr>
    <tr>
      <td id="T_formula_sheet_ab3cf35d4f5e6964_row4_col0" class="data row4 col0" >Volumes formed by rotation about the y-axis = $V=\pi \int_a^b x^2 dy$</td>
    </tr>
    <tr>
      <td id="T_formula_sheet_ab3cf35d4f5e6964_row5_col0" class="data row5 col0" >$ {\Large\int} f'(x)\cos f(x)dx = \sin f(x) + c$</td>
    </tr>
    <tr>
      <td id="T_formula_sheet_ab3cf35d4f5e6964_row6_col0" class="data row6 col0" >$ {\Large\int} f'(x)\sin f(x)dx = -\cos f(x) + c$</td>
    </tr>
    <tr>
      <td id="T_formula_sheet_ab3cf35d4f5e6964_row7_col0" class="data row7 col0" >$ {\Large\int} f'(x)\sec^2 f(x)dx = \tan f(x) + c$</td>
    </tr>
    <tr>
      <td id="T_formula_sheet_ab3cf35d4f5e6964_row8_col0" class="data row8 col0" >$ {\Large\int} f'(x)e^{f(x)}dx = e^{f(x)} + c$</td>
    </tr>
    <tr>
      <td id="T_formula_sheet_ab3cf35d4f5e6964_row9_col0" class="data row9 col0" >$ {\Large\int} \dfrac{f'(x)}{f(x)}dx = \ln|f(x)| + c$</td>
    </tr>
    <tr>
      <td id="T_formula_sheet_ab3cf35d4f5e6964_row10_col0" class="data row10 col0" >$ {\Large\int} f'(x)a^{f(x)}dx = \dfrac{a^f(x)}{\ln  a} +c$</td>
    </tr>
    <tr>
      <td id="T_formula_sheet_ab3cf35d4f5e6964_row11_col0" class="data row11 col0" >$ {\Large\int} \dfrac{f'(x)}{(\ln a) f(x)} = \log_{a} |f(x)|  + c$</td>
    </tr>
    <tr>
      <td id="T_formula_sheet_ab3cf35d4f5e6964_row12_col0" class="data row12 col0" >$ {\Large\int}_b^a f(x)dx = F(b)-F(a) \text{, where F(x) is the anti-derivative of f(x)}$</td>
    </tr>
    <tr>
      <td id="T_formula_sheet_ab3cf35d4f5e6964_row13_col0" class="data row13 col0" >$F'(x) = \dfrac{d}{dx} {\Large\int}_a^x f(t)dt = f(x) \text{ (the Fundamental Therom of Calculus)}$</td>
    </tr>
    <tr>
      <td id="T_formula_sheet_ab3cf35d4f5e6964_row14_col0" class="data row14 col0" >$ {\Large\int} \dfrac{f'(x)} {\sqrt {1 - (f(x))^2} } dx = \sin^{-1} f(x) + c$</td>
    </tr>
    <tr>
      <td id="T_formula_sheet_ab3cf35d4f5e6964_row15_col0" class="data row15 col0" >$ {\Large\int} \dfrac{f'(x)} {\sqrt {a^2 - (f(x))^2} } dx = \sin^{-1} \dfrac{f(x)}{a} + c$</td>
    </tr>
    <tr>
      <td id="T_formula_sheet_ab3cf35d4f5e6964_row16_col0" class="data row16 col0" >$ {\Large\int} - \dfrac{f'(x)} {\sqrt {1 - (f(x))^2} }  = \cos^{-1}f(x) + c \text{ or } -\sin^{-1}f(x) +c$
$ \text{Note the constant c will have different values with these two options} $</td>
    </tr>
    <tr>
      <td id="T_formula_sheet_ab3cf35d4f5e6964_row17_col0" class="data row17 col0" >$ {\Large\int} - \dfrac{f'(x)} {\sqrt {a^2 - (f(x))^2} }  = \cos^{-1}\dfrac{f(x)}{a} + c \text{ or } -\sin^{-1}\dfrac{f(x)}{a} +c$
$ \text{Note the constant c will have different values with these two options} $</td>
    </tr>
    <tr>
      <td id="T_formula_sheet_ab3cf35d4f5e6964_row18_col0" class="data row18 col0" >$ {\Large\int} \dfrac{f'(x)} {1 + (f(x))^2} dx = \ \tan^{-1} f(x) + c$</td>
    </tr>
    <tr>
      <td id="T_formula_sheet_ab3cf35d4f5e6964_row19_col0" class="data row19 col0" >$ {\Large\int} \dfrac{f'(x)} {a^2 + (f(x))^2} dx = \dfrac{1}{a} \tan^{-1} \dfrac{f(x)}{a} + c$</td>
    </tr>
  </tbody>
</table>
{{< /tab >}}

{{< tab "Proofs required" >}}

Items where proofs required are highlighted 
<br>
<style type="text/css">
#T_proof_required_7077da796d528bdb th.col_heading {
  text-align: left;
  font-size: 1em;
}
#T_proof_required_7077da796d528bdb td {
  text-align: left;
  font-size: 1em;
  padding: 1.5em;
}
#T_proof_required_7077da796d528bdb_row0_col0, #T_proof_required_7077da796d528bdb_row3_col0, #T_proof_required_7077da796d528bdb_row4_col0, #T_proof_required_7077da796d528bdb_row5_col0, #T_proof_required_7077da796d528bdb_row6_col0, #T_proof_required_7077da796d528bdb_row8_col0, #T_proof_required_7077da796d528bdb_row9_col0, #T_proof_required_7077da796d528bdb_row12_col0, #T_proof_required_7077da796d528bdb_row13_col0, #T_proof_required_7077da796d528bdb_row14_col0, #T_proof_required_7077da796d528bdb_row15_col0, #T_proof_required_7077da796d528bdb_row16_col0, #T_proof_required_7077da796d528bdb_row17_col0, #T_proof_required_7077da796d528bdb_row18_col0, #T_proof_required_7077da796d528bdb_row19_col0 {
  background-color: rgba(0,150,200, 0.2);
}
#T_proof_required_7077da796d528bdb_row1_col0, #T_proof_required_7077da796d528bdb_row2_col0, #T_proof_required_7077da796d528bdb_row7_col0, #T_proof_required_7077da796d528bdb_row10_col0, #T_proof_required_7077da796d528bdb_row11_col0 {
  background-color: rgba(0,0,0,0);
}
</style>
<table id="T_proof_required_7077da796d528bdb">
  <thead>
  </thead>
  <tbody>
    <tr>
      <td id="T_proof_required_7077da796d528bdb_row0_col0" class="data row0 col0" >$ {\Large\int} f'(x)[f(x)]^n dx = \dfrac{1}{n+1}[f(x)]^{n+1} + c $
$ \text{ where } n \neq -1 $</td>
    </tr>
    <tr>
      <td id="T_proof_required_7077da796d528bdb_row1_col0" class="data row1 col0" >$ {\Large\int} u \dfrac{dv}{dx} dx=uv-{\Large\int}v \dfrac {du}{dx}dx$</td>
    </tr>
    <tr>
      <td id="T_proof_required_7077da796d528bdb_row2_col0" class="data row2 col0" >$ {\Large\int_{a}^{b}} f(x) dx \approx \dfrac{b-a} {2n} {\Large\{} f(a) + f(b) + 2 {\Large[} f(x_1)+...+f(x_{n-1}){\Large ]} {\Large\}}$
$ \text { where } a=x_0 \text{ and } b=x_n $</td>
    </tr>
    <tr>
      <td id="T_proof_required_7077da796d528bdb_row3_col0" class="data row3 col0" >Volumes formed by rotation about the x-axis = $V=\pi \int_a^b y^2 dx$</td>
    </tr>
    <tr>
      <td id="T_proof_required_7077da796d528bdb_row4_col0" class="data row4 col0" >Volumes formed by rotation about the y-axis = $V=\pi \int_a^b x^2 dy$</td>
    </tr>
    <tr>
      <td id="T_proof_required_7077da796d528bdb_row5_col0" class="data row5 col0" >$ {\Large\int} f'(x)\cos f(x)dx = \sin f(x) + c$</td>
    </tr>
    <tr>
      <td id="T_proof_required_7077da796d528bdb_row6_col0" class="data row6 col0" >$ {\Large\int} f'(x)\sin f(x)dx = -\cos f(x) + c$</td>
    </tr>
    <tr>
      <td id="T_proof_required_7077da796d528bdb_row7_col0" class="data row7 col0" >$ {\Large\int} f'(x)\sec^2 f(x)dx = \tan f(x) + c$</td>
    </tr>
    <tr>
      <td id="T_proof_required_7077da796d528bdb_row8_col0" class="data row8 col0" >$ {\Large\int} f'(x)e^{f(x)}dx = e^{f(x)} + c$</td>
    </tr>
    <tr>
      <td id="T_proof_required_7077da796d528bdb_row9_col0" class="data row9 col0" >$ {\Large\int} \dfrac{f'(x)}{f(x)}dx = \ln|f(x)| + c$</td>
    </tr>
    <tr>
      <td id="T_proof_required_7077da796d528bdb_row10_col0" class="data row10 col0" >$ {\Large\int} f'(x)a^{f(x)}dx = \dfrac{a^f(x)}{\ln  a} +c$</td>
    </tr>
    <tr>
      <td id="T_proof_required_7077da796d528bdb_row11_col0" class="data row11 col0" >$ {\Large\int} \dfrac{f'(x)}{(\ln a) f(x)} = \log_{a} |f(x)|  + c$</td>
    </tr>
    <tr>
      <td id="T_proof_required_7077da796d528bdb_row12_col0" class="data row12 col0" >$ {\Large\int}_b^a f(x)dx = F(b)-F(a) \text{, where F(x) is the anti-derivative of f(x)}$</td>
    </tr>
    <tr>
      <td id="T_proof_required_7077da796d528bdb_row13_col0" class="data row13 col0" >$F'(x) = \dfrac{d}{dx} {\Large\int}_a^x f(t)dt = f(x) \text{ (the Fundamental Therom of Calculus)}$</td>
    </tr>
    <tr>
      <td id="T_proof_required_7077da796d528bdb_row14_col0" class="data row14 col0" >$ {\Large\int} \dfrac{f'(x)} {\sqrt {1 - (f(x))^2} } dx = \sin^{-1} f(x) + c$</td>
    </tr>
    <tr>
      <td id="T_proof_required_7077da796d528bdb_row15_col0" class="data row15 col0" >$ {\Large\int} \dfrac{f'(x)} {\sqrt {a^2 - (f(x))^2} } dx = \sin^{-1} \dfrac{f(x)}{a} + c$</td>
    </tr>
    <tr>
      <td id="T_proof_required_7077da796d528bdb_row16_col0" class="data row16 col0" >$ {\Large\int} - \dfrac{f'(x)} {\sqrt {1 - (f(x))^2} }  = \cos^{-1}f(x) + c \text{ or } -\sin^{-1}f(x) +c$
$ \text{Note the constant c will have different values with these two options} $</td>
    </tr>
    <tr>
      <td id="T_proof_required_7077da796d528bdb_row17_col0" class="data row17 col0" >$ {\Large\int} - \dfrac{f'(x)} {\sqrt {a^2 - (f(x))^2} }  = \cos^{-1}\dfrac{f(x)}{a} + c \text{ or } -\sin^{-1}\dfrac{f(x)}{a} +c$
$ \text{Note the constant c will have different values with these two options} $</td>
    </tr>
    <tr>
      <td id="T_proof_required_7077da796d528bdb_row18_col0" class="data row18 col0" >$ {\Large\int} \dfrac{f'(x)} {1 + (f(x))^2} dx = \ \tan^{-1} f(x) + c$</td>
    </tr>
    <tr>
      <td id="T_proof_required_7077da796d528bdb_row19_col0" class="data row19 col0" >$ {\Large\int} \dfrac{f'(x)} {a^2 + (f(x))^2} dx = \dfrac{1}{a} \tan^{-1} \dfrac{f(x)}{a} + c$</td>
    </tr>
  </tbody>
</table>
{{< /tab >}}
{{< /tabs >}}