---
weight: 5
---

{{< tabs "uniqueid" >}}

{{< tab "Standard view" >}}

<style type="text/css">
#T_4936e th.col_heading {
  text-align: left;
  font-size: 1em;
}
#T_4936e td {
  text-align: left;
  font-size: 1em;
  padding: 1.5em;
}
#T_4936e_row0_col0, #T_4936e_row1_col0, #T_4936e_row2_col0, #T_4936e_row3_col0, #T_4936e_row4_col0, #T_4936e_row5_col0, #T_4936e_row6_col0, #T_4936e_row7_col0, #T_4936e_row8_col0, #T_4936e_row9_col0, #T_4936e_row10_col0, #T_4936e_row11_col0, #T_4936e_row12_col0, #T_4936e_row13_col0, #T_4936e_row14_col0, #T_4936e_row15_col0, #T_4936e_row16_col0, #T_4936e_row17_col0, #T_4936e_row18_col0, #T_4936e_row19_col0, #T_4936e_row20_col0, #T_4936e_row21_col0, #T_4936e_row22_col0, #T_4936e_row23_col0, #T_4936e_row24_col0 {
  width: 400px;
  white-space: pre-wrap;
}
</style>
<table id="T_4936e">
  <thead>
  </thead>
  <tbody>
    <tr>
      <td id="T_4936e_row0_col0" class="data row0 col0" >$ y=f(x)   \,\,\,\,\,\,\,\,\,\,\,\,\,\,\,\,\,\,\,\,\,\,\,\,\,\,\,\,\,\,\,\,\,\,\,\,\,\,\,\,\,\,\,\,\,\,\,\,\,\,   \dfrac{dy}{dx} =\lim\limits_{h \to 0} \dfrac{f(x+h) - f(x)}{h}  $ <br></td>
    </tr>
    <tr>
      <td id="T_4936e_row1_col0" class="data row1 col0" >$ y=kx   \,\,\,\,\,\,\,\,\,\,\,\,\,\,\,\,\,\,\,\,\,\,\,\,\,\,\,\,\,\,\,\,\,\,\,\,\,\,\,\,\,\,\,\,\,\,\,\,\,\,\,\,\,\,\,   \dfrac{dy}{dx} =k  $ <br></td>
    </tr>
    <tr>
      <td id="T_4936e_row2_col0" class="data row2 col0" >$ y=k   \,\,\,\,\,\,\,\,\,\,\,\,\,\,\,\,\,\,\,\,\,\,\,\,\,\,\,\,\,\,\,\,\,\,\,\,\,\,\,\,\,\,\,\,\,\,\,\,\,\,\,\,\,\,\,\,\,\,\,   \dfrac{dy}{dx} =0  $ <br></td>
    </tr>
    <tr>
      <td id="T_4936e_row3_col0" class="data row3 col0" >$ y=x^n   \,\,\,\,\,\,\,\,\,\,\,\,\,\,\,\,\,\,\,\,\,\,\,\,\,\,\,\,\,\,\,\,\,\,\,\,\,\,\,\,\,\,\,\,\,\,\,\,\,\,\,\,\,\,\,\,   \dfrac{dy}{dx} =nx^{n-1}  $ <br></td>
    </tr>
    <tr>
      <td id="T_4936e_row4_col0" class="data row4 col0" >$ y=kx^n   \,\,\,\,\,\,\,\,\,\,\,\,\,\,\,\,\,\,\,\,\,\,\,\,\,\,\,\,\,\,\,\,\,\,\,\,\,\,\,\,\,\,\,\,\,\,\,\,\,\,\,\,\,   \dfrac{dy}{dx} =knx^{n-1}  $ <br></td>
    </tr>
    <tr>
      <td id="T_4936e_row5_col0" class="data row5 col0" >$ y=kf(x)   \,\,\,\,\,\,\,\,\,\,\,\,\,\,\,\,\,\,\,\,\,\,\,\,\,\,\,\,\,\,\,\,\,\,\,\,\,\,\,\,\,\,\,\,\,\,\,\,   \dfrac{dy}{dx} =kf'(x)  $ <br></td>
    </tr>
    <tr>
      <td id="T_4936e_row6_col0" class="data row6 col0" >$ y=f(x) + g(x)   \,\,\,\,\,\,\,\,\,\,\,\,\,\,\,\,\,\,\,\,\,\,\,\,\,\,\,\,\,\,\,\,\,   \dfrac{dy}{dx} =f'(x) + g'(x)  $ <br></td>
    </tr>
    <tr>
      <td id="T_4936e_row7_col0" class="data row7 col0" >$y=f(x)^n \,\,\,\,\,\,\,\,\,\,\,\,\,\,\,\,\,\,\,\,\,\,\,\,\,\,\,\,\,\,\,\,\,\,\,\,\,\,\,\,\,\,\,\,\,\,\,\,  \dfrac{dy}{dx}=nf'(x)[f(x)]^{n-1}$ <br></td>
    </tr>
    <tr>
      <td id="T_4936e_row8_col0" class="data row8 col0" >$y=uv \,\,\,\,\,\,\,\,\,\,\,\,\,\,\,\,\,\,\,\,\,\,\,\,\,\,\,\,\,\,\,\,\,\,\,\,\,\,\,\,\,\,\,\,\,\,\,\,\,\,\,\,\,\,\,\,   \dfrac{dy}{dx} = u\dfrac{dv}{dx} + v\dfrac{du}{dx}$ <br></td>
    </tr>
    <tr>
      <td id="T_4936e_row9_col0" class="data row9 col0" >$y=\dfrac{u}{v} \,\,\,\,\,\,\,\,\,\,\,\,\,\,\,\,\,\,\,\,\,\,\,\,\,\,\,\,\,\,\,\,\,\,\,\,\,\,\,\,\,\,\,\,\,\,\,\,\,\,\,\,\,\,\,\,   \dfrac{dy}{dx} = \dfrac{v\dfrac{du}{dx} - u\dfrac{dv}{dx}}{v^2}$ <br></td>
    </tr>
    <tr>
      <td id="T_4936e_row10_col0" class="data row10 col0" >$y=g(u) \text { where } u = f(x) \,\,\,\,\,\,\,\,\,\,   \dfrac{dy}{dx} = \dfrac{dy}{du} \times \dfrac{du}{dx}$ <br></td>
    </tr>
    <tr>
      <td id="T_4936e_row11_col0" class="data row11 col0" >$y=sinf(x) \,\,\,\,\,\,\,\,\,\,\,\,\,\,\,\,\,\,\,\,\,\,\,\,\,\,\,\,\,\,\,\,\,\,\,\,\,\,\,\,\,\,  \dfrac{dy}{dx} = f'(x)cos f(x)$ <br></td>
    </tr>
    <tr>
      <td id="T_4936e_row12_col0" class="data row12 col0" >$y=cosf(x) \,\,\,\,\,\,\,\,\,\,\,\,\,\,\,\,\,\,\,\,\,\,\,\,\,\,\,\,\,\,\,\,\,\,\,\,\,\,\,\,\,\,\,   \dfrac{dy}{dx} = -f'(x)sin f(x)$ <br></td>
    </tr>
    <tr>
      <td id="T_4936e_row13_col0" class="data row13 col0" >$y=tan f(x) \,\,\,\,\,\,\,\,\,\,\,\,\,\,\,\,\,\,\,\,\,\,\,\,\,\,\,\,\,\,\,\,\,\,\,\,\,\,\,\,\,\,   \dfrac{dy}{dx} = f'(x)sec^2 f(x)$ <br></td>
    </tr>
    <tr>
      <td id="T_4936e_row14_col0" class="data row14 col0" >$y=e^{f(x)} \,\,\,\,\,\,\,\,\,\,\,\,\,\,\,\,\,\,\,\,\,\,\,\,\,\,\,\,\,\,\,\,\,\,\,\,\,\,\,\,\,\,\,\,\,\,\,\,\,\,\,   \dfrac{dy}{dx} = f'(x) e^{f(x)}$ <br></td>
    </tr>
    <tr>
      <td id="T_4936e_row15_col0" class="data row15 col0" >$y=\ln f(x) \,\,\,\,\,\,\,\,\,\,\,\,\,\,\,\,\,\,\,\,\,\,\,\,\,\,\,\,\,\,\,\,\,\,\,\,\,\,\,\,\,\,\,\,\,   \dfrac{dy}{dx} = \dfrac{f'(x)}{f(x)}$ <br></td>
    </tr>
    <tr>
      <td id="T_4936e_row16_col0" class="data row16 col0" >$y=a^{f(x)} \,\,\,\,\,\,\,\,\,\,\,\,\,\,\,\,\,\,\,\,\,\,\,\,\,\,\,\,\,\,\,\,\,\,\,\,\,\,\,\,\,\,\,\,\,\,\,\,\,\,\,   \dfrac{dy}{dx} = (\ln a)f'(x)a^{f(x)}$ <br></td>
    </tr>
    <tr>
      <td id="T_4936e_row17_col0" class="data row17 col0" >$y=log _{a} f(x) \,\,\,\,\,\,\,\,\,\,\,\,\,\,\,\,\,\,\,\,\,\,\,\,\,\,\,\,\,\,\,\,\,\,\,\,\,\,\,\,\,   \dfrac{dy}{dx} = \dfrac{f'(x)}{(\ln a) f(x)}$ <br></td>
    </tr>
    <tr>
      <td id="T_4936e_row18_col0" class="data row18 col0" >$y=sin^{-1}f(x) \,\,\,\,\,\,\,\,\,\,\,\,\,\,\,\,\,\,\,\,\,\,\,\,\,\,\,\,\,\,\,\,\,\,\,\,\,   \dfrac{dy}{dx} = \dfrac{f'(x)} {\sqrt {1 - (f(x))^2} }$ <br></td>
    </tr>
    <tr>
      <td id="T_4936e_row19_col0" class="data row19 col0" >$ y = sin^{-1} \dfrac{f(x)}{a}  \,\,\,\,\,\,\,\,\,\,\,\,\,\,\,\,\,\,\,\,\,\,\,\,\,\,\,\,\,\,\,\,\,\,\,   \dfrac{dy}{dx} = \dfrac{f'(x)}{\sqrt{a^2 - (f(x))^2}} $ <br></td>
    </tr>
    <tr>
      <td id="T_4936e_row20_col0" class="data row20 col0" >$y=cos^{-1}f(x) \,\,\,\,\,\,\,\,\,\,\,\,\,\,\,\,\,\,\,\,\,\,\,\,\,\,\,\,\,\,\,\,\,\,\,\,\,   \dfrac{dy}{dx} = - \dfrac{f'(x)} {\sqrt {1 - (f(x))^2} }$ <br></td>
    </tr>
    <tr>
      <td id="T_4936e_row21_col0" class="data row21 col0" >$y=cos^{-1} \dfrac{f(x)}{a} \,\,\,\,\,\,\,\,\,\,\,\,\,\,\,\,\,\,\,\,\,\,\,\,\,\,\,\,\,\,\,\,\,\,\,   \dfrac{dy}{dx} = - \dfrac{f'(x)} {\sqrt {a^2 - (f(x))^2} }$ <br></td>
    </tr>
    <tr>
      <td id="T_4936e_row22_col0" class="data row22 col0" >$y=tan^{-1}f(x) \,\,\,\,\,\,\,\,\,\,\,\,\,\,\,\,\,\,\,\,\,\,\,\,\,\,\,\,\,\,\,\,\,\,\,\,\,   \dfrac{dy}{dx} = \dfrac{f'(x)} {1 + (f(x))^2}$ <br></td>
    </tr>
    <tr>
      <td id="T_4936e_row23_col0" class="data row23 col0" >$y=tan^{-1}\dfrac{f(x)}{a} \,\,\,\,\,\,\,\,\,\,\,\,\,\,\,\,\,\,\,\,\,\,\,\,\,\,\,\,\,\,\,\,\,\,\,   \dfrac{dy}{dx} =  \dfrac{1}{a} tan^{-1} \dfrac{f(x)}{a} $ <br></td>
    </tr>
    <tr>
      <td id="T_4936e_row24_col0" class="data row24 col0" >$ \text{Function and its inverse}  \,\,\,\,\,\,\,\,\,\,\,\,\,   \dfrac{dy}{dx} \times \dfrac{dx}{dy} = 1, \text{  or  } \dfrac{dy}{dx} = \dfrac{1}{\dfrac{dx}{dy}} $ <br></td>
    </tr>
  </tbody>
</table>
{{< /tab >}}

{{< tab "Formula sheet" >}}Items on formula sheet are highlighted
<br>
<style type="text/css">
#T_6866c th.col_heading {
  text-align: left;
  font-size: 1em;
}
#T_6866c td {
  text-align: left;
  font-size: 1em;
  padding: 1.5em;
}
#T_6866c_row0_col0, #T_6866c_row1_col0, #T_6866c_row2_col0, #T_6866c_row3_col0, #T_6866c_row4_col0, #T_6866c_row5_col0, #T_6866c_row6_col0, #T_6866c_row19_col0, #T_6866c_row21_col0, #T_6866c_row23_col0, #T_6866c_row24_col0 {
  width: 400px;
  white-space: pre-wrap;
}
#T_6866c_row7_col0, #T_6866c_row8_col0, #T_6866c_row9_col0, #T_6866c_row10_col0, #T_6866c_row11_col0, #T_6866c_row12_col0, #T_6866c_row13_col0, #T_6866c_row14_col0, #T_6866c_row15_col0, #T_6866c_row16_col0, #T_6866c_row17_col0, #T_6866c_row18_col0, #T_6866c_row20_col0, #T_6866c_row22_col0 {
  width: 400px;
  background-color: rgba(255,194,10, 0.2);
  white-space: pre-wrap;
}
</style>
<table id="T_6866c">
  <thead>
  </thead>
  <tbody>
    <tr>
      <td id="T_6866c_row0_col0" class="data row0 col0" >$ y=f(x)   \,\,\,\,\,\,\,\,\,\,\,\,\,\,\,\,\,\,\,\,\,\,\,\,\,\,\,\,\,\,\,\,\,\,\,\,\,\,\,\,\,\,\,\,\,\,\,\,\,\,   \dfrac{dy}{dx} =\lim\limits_{h \to 0} \dfrac{f(x+h) - f(x)}{h}  $ <br></td>
    </tr>
    <tr>
      <td id="T_6866c_row1_col0" class="data row1 col0" >$ y=kx   \,\,\,\,\,\,\,\,\,\,\,\,\,\,\,\,\,\,\,\,\,\,\,\,\,\,\,\,\,\,\,\,\,\,\,\,\,\,\,\,\,\,\,\,\,\,\,\,\,\,\,\,\,\,\,   \dfrac{dy}{dx} =k  $ <br></td>
    </tr>
    <tr>
      <td id="T_6866c_row2_col0" class="data row2 col0" >$ y=k   \,\,\,\,\,\,\,\,\,\,\,\,\,\,\,\,\,\,\,\,\,\,\,\,\,\,\,\,\,\,\,\,\,\,\,\,\,\,\,\,\,\,\,\,\,\,\,\,\,\,\,\,\,\,\,\,\,\,\,   \dfrac{dy}{dx} =0  $ <br></td>
    </tr>
    <tr>
      <td id="T_6866c_row3_col0" class="data row3 col0" >$ y=x^n   \,\,\,\,\,\,\,\,\,\,\,\,\,\,\,\,\,\,\,\,\,\,\,\,\,\,\,\,\,\,\,\,\,\,\,\,\,\,\,\,\,\,\,\,\,\,\,\,\,\,\,\,\,\,\,\,   \dfrac{dy}{dx} =nx^{n-1}  $ <br></td>
    </tr>
    <tr>
      <td id="T_6866c_row4_col0" class="data row4 col0" >$ y=kx^n   \,\,\,\,\,\,\,\,\,\,\,\,\,\,\,\,\,\,\,\,\,\,\,\,\,\,\,\,\,\,\,\,\,\,\,\,\,\,\,\,\,\,\,\,\,\,\,\,\,\,\,\,\,   \dfrac{dy}{dx} =knx^{n-1}  $ <br></td>
    </tr>
    <tr>
      <td id="T_6866c_row5_col0" class="data row5 col0" >$ y=kf(x)   \,\,\,\,\,\,\,\,\,\,\,\,\,\,\,\,\,\,\,\,\,\,\,\,\,\,\,\,\,\,\,\,\,\,\,\,\,\,\,\,\,\,\,\,\,\,\,\,   \dfrac{dy}{dx} =kf'(x)  $ <br></td>
    </tr>
    <tr>
      <td id="T_6866c_row6_col0" class="data row6 col0" >$ y=f(x) + g(x)   \,\,\,\,\,\,\,\,\,\,\,\,\,\,\,\,\,\,\,\,\,\,\,\,\,\,\,\,\,\,\,\,\,   \dfrac{dy}{dx} =f'(x) + g'(x)  $ <br></td>
    </tr>
    <tr>
      <td id="T_6866c_row7_col0" class="data row7 col0" >$y=f(x)^n \,\,\,\,\,\,\,\,\,\,\,\,\,\,\,\,\,\,\,\,\,\,\,\,\,\,\,\,\,\,\,\,\,\,\,\,\,\,\,\,\,\,\,\,\,\,\,\,  \dfrac{dy}{dx}=nf'(x)[f(x)]^{n-1}$ <br></td>
    </tr>
    <tr>
      <td id="T_6866c_row8_col0" class="data row8 col0" >$y=uv \,\,\,\,\,\,\,\,\,\,\,\,\,\,\,\,\,\,\,\,\,\,\,\,\,\,\,\,\,\,\,\,\,\,\,\,\,\,\,\,\,\,\,\,\,\,\,\,\,\,\,\,\,\,\,\,   \dfrac{dy}{dx} = u\dfrac{dv}{dx} + v\dfrac{du}{dx}$ <br></td>
    </tr>
    <tr>
      <td id="T_6866c_row9_col0" class="data row9 col0" >$y=\dfrac{u}{v} \,\,\,\,\,\,\,\,\,\,\,\,\,\,\,\,\,\,\,\,\,\,\,\,\,\,\,\,\,\,\,\,\,\,\,\,\,\,\,\,\,\,\,\,\,\,\,\,\,\,\,\,\,\,\,\,   \dfrac{dy}{dx} = \dfrac{v\dfrac{du}{dx} - u\dfrac{dv}{dx}}{v^2}$ <br></td>
    </tr>
    <tr>
      <td id="T_6866c_row10_col0" class="data row10 col0" >$y=g(u) \text { where } u = f(x) \,\,\,\,\,\,\,\,\,\,   \dfrac{dy}{dx} = \dfrac{dy}{du} \times \dfrac{du}{dx}$ <br></td>
    </tr>
    <tr>
      <td id="T_6866c_row11_col0" class="data row11 col0" >$y=sinf(x) \,\,\,\,\,\,\,\,\,\,\,\,\,\,\,\,\,\,\,\,\,\,\,\,\,\,\,\,\,\,\,\,\,\,\,\,\,\,\,\,\,\,  \dfrac{dy}{dx} = f'(x)cos f(x)$ <br></td>
    </tr>
    <tr>
      <td id="T_6866c_row12_col0" class="data row12 col0" >$y=cosf(x) \,\,\,\,\,\,\,\,\,\,\,\,\,\,\,\,\,\,\,\,\,\,\,\,\,\,\,\,\,\,\,\,\,\,\,\,\,\,\,\,\,\,\,   \dfrac{dy}{dx} = -f'(x)sin f(x)$ <br></td>
    </tr>
    <tr>
      <td id="T_6866c_row13_col0" class="data row13 col0" >$y=tan f(x) \,\,\,\,\,\,\,\,\,\,\,\,\,\,\,\,\,\,\,\,\,\,\,\,\,\,\,\,\,\,\,\,\,\,\,\,\,\,\,\,\,\,   \dfrac{dy}{dx} = f'(x)sec^2 f(x)$ <br></td>
    </tr>
    <tr>
      <td id="T_6866c_row14_col0" class="data row14 col0" >$y=e^{f(x)} \,\,\,\,\,\,\,\,\,\,\,\,\,\,\,\,\,\,\,\,\,\,\,\,\,\,\,\,\,\,\,\,\,\,\,\,\,\,\,\,\,\,\,\,\,\,\,\,\,\,\,   \dfrac{dy}{dx} = f'(x) e^{f(x)}$ <br></td>
    </tr>
    <tr>
      <td id="T_6866c_row15_col0" class="data row15 col0" >$y=\ln f(x) \,\,\,\,\,\,\,\,\,\,\,\,\,\,\,\,\,\,\,\,\,\,\,\,\,\,\,\,\,\,\,\,\,\,\,\,\,\,\,\,\,\,\,\,\,   \dfrac{dy}{dx} = \dfrac{f'(x)}{f(x)}$ <br></td>
    </tr>
    <tr>
      <td id="T_6866c_row16_col0" class="data row16 col0" >$y=a^{f(x)} \,\,\,\,\,\,\,\,\,\,\,\,\,\,\,\,\,\,\,\,\,\,\,\,\,\,\,\,\,\,\,\,\,\,\,\,\,\,\,\,\,\,\,\,\,\,\,\,\,\,\,   \dfrac{dy}{dx} = (\ln a)f'(x)a^{f(x)}$ <br></td>
    </tr>
    <tr>
      <td id="T_6866c_row17_col0" class="data row17 col0" >$y=log _{a} f(x) \,\,\,\,\,\,\,\,\,\,\,\,\,\,\,\,\,\,\,\,\,\,\,\,\,\,\,\,\,\,\,\,\,\,\,\,\,\,\,\,\,   \dfrac{dy}{dx} = \dfrac{f'(x)}{(\ln a) f(x)}$ <br></td>
    </tr>
    <tr>
      <td id="T_6866c_row18_col0" class="data row18 col0" >$y=sin^{-1}f(x) \,\,\,\,\,\,\,\,\,\,\,\,\,\,\,\,\,\,\,\,\,\,\,\,\,\,\,\,\,\,\,\,\,\,\,\,\,   \dfrac{dy}{dx} = \dfrac{f'(x)} {\sqrt {1 - (f(x))^2} }$ <br></td>
    </tr>
    <tr>
      <td id="T_6866c_row19_col0" class="data row19 col0" >$ y = sin^{-1} \dfrac{f(x)}{a}  \,\,\,\,\,\,\,\,\,\,\,\,\,\,\,\,\,\,\,\,\,\,\,\,\,\,\,\,\,\,\,\,\,\,\,   \dfrac{dy}{dx} = \dfrac{f'(x)}{\sqrt{a^2 - (f(x))^2}} $ <br></td>
    </tr>
    <tr>
      <td id="T_6866c_row20_col0" class="data row20 col0" >$y=cos^{-1}f(x) \,\,\,\,\,\,\,\,\,\,\,\,\,\,\,\,\,\,\,\,\,\,\,\,\,\,\,\,\,\,\,\,\,\,\,\,\,   \dfrac{dy}{dx} = - \dfrac{f'(x)} {\sqrt {1 - (f(x))^2} }$ <br></td>
    </tr>
    <tr>
      <td id="T_6866c_row21_col0" class="data row21 col0" >$y=cos^{-1} \dfrac{f(x)}{a} \,\,\,\,\,\,\,\,\,\,\,\,\,\,\,\,\,\,\,\,\,\,\,\,\,\,\,\,\,\,\,\,\,\,\,   \dfrac{dy}{dx} = - \dfrac{f'(x)} {\sqrt {a^2 - (f(x))^2} }$ <br></td>
    </tr>
    <tr>
      <td id="T_6866c_row22_col0" class="data row22 col0" >$y=tan^{-1}f(x) \,\,\,\,\,\,\,\,\,\,\,\,\,\,\,\,\,\,\,\,\,\,\,\,\,\,\,\,\,\,\,\,\,\,\,\,\,   \dfrac{dy}{dx} = \dfrac{f'(x)} {1 + (f(x))^2}$ <br></td>
    </tr>
    <tr>
      <td id="T_6866c_row23_col0" class="data row23 col0" >$y=tan^{-1}\dfrac{f(x)}{a} \,\,\,\,\,\,\,\,\,\,\,\,\,\,\,\,\,\,\,\,\,\,\,\,\,\,\,\,\,\,\,\,\,\,\,   \dfrac{dy}{dx} =  \dfrac{1}{a} tan^{-1} \dfrac{f(x)}{a} $ <br></td>
    </tr>
    <tr>
      <td id="T_6866c_row24_col0" class="data row24 col0" >$ \text{Function and its inverse}  \,\,\,\,\,\,\,\,\,\,\,\,\,   \dfrac{dy}{dx} \times \dfrac{dx}{dy} = 1, \text{  or  } \dfrac{dy}{dx} = \dfrac{1}{\dfrac{dx}{dy}} $ <br></td>
    </tr>
  </tbody>
</table>
{{< /tab >}}
{{< /tabs >}}