---
---

# TBA

<br>

## Definitions

These are the definitions

<br>

## Formulas

{{< tabs "uniqueid" >}}

{{< tab "Standard view" >}}

<style type="text/css">
#T_687be th.col_heading {
  text-align: left;
  font-size: 1em;
}
#T_687be td {
  text-align: left;
  font-size: 1em;
  padding: 1.5em;
}
#T_687be_row0_col0, #T_687be_row1_col0, #T_687be_row2_col0, #T_687be_row3_col0, #T_687be_row4_col0, #T_687be_row5_col0, #T_687be_row6_col0, #T_687be_row7_col0, #T_687be_row8_col0, #T_687be_row9_col0, #T_687be_row10_col0, #T_687be_row11_col0, #T_687be_row12_col0 {
  width: 400px;
  white-space: pre-wrap;
}
</style>
<table id="T_687be">
  <thead>
  </thead>
  <tbody>
    <tr>
      <td id="T_687be_row0_col0" class="data row0 col0" >$y=sin^{-1}f(x) \,\,\,\,\,\,\,\,\,\,\,\,\,\,\,\,\,\,\,\,\,\,\,\,\,\,\,\,\,\,\,\,\,\,\,\,\,   \dfrac{dy}{dx} = \dfrac{f'(x)} {\sqrt {1 - (f(x))^2} }$ <br></td>
    </tr>
    <tr>
      <td id="T_687be_row1_col0" class="data row1 col0" >$ {\Large\int} \dfrac{f'(x)} {\sqrt {1 - (f(x))^2} } dx = sin^{-1} f(x) + c$</td>
    </tr>
    <tr>
      <td id="T_687be_row2_col0" class="data row2 col0" >$ y = sin^{-1} \dfrac{f(x)}{a}  \,\,\,\,\,\,\,\,\,\,\,\,\,\,\,\,\,\,\,\,\,\,\,\,\,\,\,\,\,\,\,\,\,\,\,   \dfrac{dy}{dx} = \dfrac{f'(x)}{\sqrt{a^2 - (f(x))^2}} $ <br></td>
    </tr>
    <tr>
      <td id="T_687be_row3_col0" class="data row3 col0" >$ {\Large\int} \dfrac{f'(x)} {\sqrt {a^2 - (f(x))^2} } dx = sin^{-1} \dfrac{f(x)}{a} + c$</td>
    </tr>
    <tr>
      <td id="T_687be_row4_col0" class="data row4 col0" >$y=cos^{-1}f(x) \,\,\,\,\,\,\,\,\,\,\,\,\,\,\,\,\,\,\,\,\,\,\,\,\,\,\,\,\,\,\,\,\,\,\,\,\,   \dfrac{dy}{dx} = - \dfrac{f'(x)} {\sqrt {1 - (f(x))^2} }$ <br></td>
    </tr>
    <tr>
      <td id="T_687be_row5_col0" class="data row5 col0" >$ {\Large\int} - \dfrac{f'(x)} {\sqrt {1 - (f(x))^2} }  = cos^{-1}f(x) + c \text{ or } -sin^{-1}f(x) +c$
$ \text{Note the constant c will have different values with these two options} $</td>
    </tr>
    <tr>
      <td id="T_687be_row6_col0" class="data row6 col0" >$y=cos^{-1} \dfrac{f(x)}{a} \,\,\,\,\,\,\,\,\,\,\,\,\,\,\,\,\,\,\,\,\,\,\,\,\,\,\,\,\,\,\,\,\,\,\,   \dfrac{dy}{dx} = - \dfrac{f'(x)} {\sqrt {a^2 - (f(x))^2} }$ <br></td>
    </tr>
    <tr>
      <td id="T_687be_row7_col0" class="data row7 col0" >$ {\Large\int} - \dfrac{f'(x)} {\sqrt {a^2 - (f(x))^2} }  = cos^{-1}\dfrac{f(x)}{a} + c \text{ or } -sin^{-1}\dfrac{f(x)}{a} +c$
$ \text{Note the constant c will have different values with these two options} $</td>
    </tr>
    <tr>
      <td id="T_687be_row8_col0" class="data row8 col0" >$y=tan^{-1}f(x) \,\,\,\,\,\,\,\,\,\,\,\,\,\,\,\,\,\,\,\,\,\,\,\,\,\,\,\,\,\,\,\,\,\,\,\,\,   \dfrac{dy}{dx} = \dfrac{f'(x)} {1 + (f(x))^2}$ <br></td>
    </tr>
    <tr>
      <td id="T_687be_row9_col0" class="data row9 col0" >$ {\Large\int} \dfrac{f'(x)} {1 + (f(x))^2} dx = \ tan^{-1} f(x) + c$</td>
    </tr>
    <tr>
      <td id="T_687be_row10_col0" class="data row10 col0" >$y=tan^{-1}\dfrac{f(x)}{a} \,\,\,\,\,\,\,\,\,\,\,\,\,\,\,\,\,\,\,\,\,\,\,\,\,\,\,\,\,\,\,\,\,\,\,   \dfrac{dy}{dx} =  \dfrac{1}{a} tan^{-1} \dfrac{f(x)}{a} $ <br></td>
    </tr>
    <tr>
      <td id="T_687be_row11_col0" class="data row11 col0" >$ {\Large\int} \dfrac{f'(x)} {a^2 + (f(x))^2} dx = \dfrac{1}{a} tan^{-1} \dfrac{f(x)}{a} + c$</td>
    </tr>
    <tr>
      <td id="T_687be_row12_col0" class="data row12 col0" >$ \text{Function and its inverse}  \,\,\,\,\,\,\,\,\,\,\,\,\,   \dfrac{dy}{dx} \times \dfrac{dx}{dy} = 1, \text{  or  } \dfrac{dy}{dx} = \dfrac{1}{\dfrac{dx}{dy}} $ <br></td>
    </tr>
  </tbody>
</table>
{{< /tab >}}

{{< tab "Formula sheet" >}}Items on formula sheet are highlighted
<br>
<style type="text/css">
#T_44d14 th.col_heading {
  text-align: left;
  font-size: 1em;
}
#T_44d14 td {
  text-align: left;
  font-size: 1em;
  padding: 1.5em;
}
#T_44d14_row0_col0, #T_44d14_row3_col0, #T_44d14_row4_col0, #T_44d14_row8_col0, #T_44d14_row11_col0 {
  width: 400px;
  background-color: rgba(255,194,10, 0.2);
  white-space: pre-wrap;
}
#T_44d14_row1_col0, #T_44d14_row2_col0, #T_44d14_row5_col0, #T_44d14_row6_col0, #T_44d14_row7_col0, #T_44d14_row9_col0, #T_44d14_row10_col0, #T_44d14_row12_col0 {
  width: 400px;
  white-space: pre-wrap;
}
</style>
<table id="T_44d14">
  <thead>
  </thead>
  <tbody>
    <tr>
      <td id="T_44d14_row0_col0" class="data row0 col0" >$y=sin^{-1}f(x) \,\,\,\,\,\,\,\,\,\,\,\,\,\,\,\,\,\,\,\,\,\,\,\,\,\,\,\,\,\,\,\,\,\,\,\,\,   \dfrac{dy}{dx} = \dfrac{f'(x)} {\sqrt {1 - (f(x))^2} }$ <br></td>
    </tr>
    <tr>
      <td id="T_44d14_row1_col0" class="data row1 col0" >$ {\Large\int} \dfrac{f'(x)} {\sqrt {1 - (f(x))^2} } dx = sin^{-1} f(x) + c$</td>
    </tr>
    <tr>
      <td id="T_44d14_row2_col0" class="data row2 col0" >$ y = sin^{-1} \dfrac{f(x)}{a}  \,\,\,\,\,\,\,\,\,\,\,\,\,\,\,\,\,\,\,\,\,\,\,\,\,\,\,\,\,\,\,\,\,\,\,   \dfrac{dy}{dx} = \dfrac{f'(x)}{\sqrt{a^2 - (f(x))^2}} $ <br></td>
    </tr>
    <tr>
      <td id="T_44d14_row3_col0" class="data row3 col0" >$ {\Large\int} \dfrac{f'(x)} {\sqrt {a^2 - (f(x))^2} } dx = sin^{-1} \dfrac{f(x)}{a} + c$</td>
    </tr>
    <tr>
      <td id="T_44d14_row4_col0" class="data row4 col0" >$y=cos^{-1}f(x) \,\,\,\,\,\,\,\,\,\,\,\,\,\,\,\,\,\,\,\,\,\,\,\,\,\,\,\,\,\,\,\,\,\,\,\,\,   \dfrac{dy}{dx} = - \dfrac{f'(x)} {\sqrt {1 - (f(x))^2} }$ <br></td>
    </tr>
    <tr>
      <td id="T_44d14_row5_col0" class="data row5 col0" >$ {\Large\int} - \dfrac{f'(x)} {\sqrt {1 - (f(x))^2} }  = cos^{-1}f(x) + c \text{ or } -sin^{-1}f(x) +c$
$ \text{Note the constant c will have different values with these two options} $</td>
    </tr>
    <tr>
      <td id="T_44d14_row6_col0" class="data row6 col0" >$y=cos^{-1} \dfrac{f(x)}{a} \,\,\,\,\,\,\,\,\,\,\,\,\,\,\,\,\,\,\,\,\,\,\,\,\,\,\,\,\,\,\,\,\,\,\,   \dfrac{dy}{dx} = - \dfrac{f'(x)} {\sqrt {a^2 - (f(x))^2} }$ <br></td>
    </tr>
    <tr>
      <td id="T_44d14_row7_col0" class="data row7 col0" >$ {\Large\int} - \dfrac{f'(x)} {\sqrt {a^2 - (f(x))^2} }  = cos^{-1}\dfrac{f(x)}{a} + c \text{ or } -sin^{-1}\dfrac{f(x)}{a} +c$
$ \text{Note the constant c will have different values with these two options} $</td>
    </tr>
    <tr>
      <td id="T_44d14_row8_col0" class="data row8 col0" >$y=tan^{-1}f(x) \,\,\,\,\,\,\,\,\,\,\,\,\,\,\,\,\,\,\,\,\,\,\,\,\,\,\,\,\,\,\,\,\,\,\,\,\,   \dfrac{dy}{dx} = \dfrac{f'(x)} {1 + (f(x))^2}$ <br></td>
    </tr>
    <tr>
      <td id="T_44d14_row9_col0" class="data row9 col0" >$ {\Large\int} \dfrac{f'(x)} {1 + (f(x))^2} dx = \ tan^{-1} f(x) + c$</td>
    </tr>
    <tr>
      <td id="T_44d14_row10_col0" class="data row10 col0" >$y=tan^{-1}\dfrac{f(x)}{a} \,\,\,\,\,\,\,\,\,\,\,\,\,\,\,\,\,\,\,\,\,\,\,\,\,\,\,\,\,\,\,\,\,\,\,   \dfrac{dy}{dx} =  \dfrac{1}{a} tan^{-1} \dfrac{f(x)}{a} $ <br></td>
    </tr>
    <tr>
      <td id="T_44d14_row11_col0" class="data row11 col0" >$ {\Large\int} \dfrac{f'(x)} {a^2 + (f(x))^2} dx = \dfrac{1}{a} tan^{-1} \dfrac{f(x)}{a} + c$</td>
    </tr>
    <tr>
      <td id="T_44d14_row12_col0" class="data row12 col0" >$ \text{Function and its inverse}  \,\,\,\,\,\,\,\,\,\,\,\,\,   \dfrac{dy}{dx} \times \dfrac{dx}{dy} = 1, \text{  or  } \dfrac{dy}{dx} = \dfrac{1}{\dfrac{dx}{dy}} $ <br></td>
    </tr>
  </tbody>
</table>
{{< /tab >}}
{{< /tabs >}}