---
weight: 4
title: 'Introduction to Differentiation'
---

## Introduction to Differentiation

###   Concepts 

- acceleration
- average rate of change
- chain rule
- derivative function
- differentiability
- differentiation
- differentiation from first principles
- displacement
- gradient of a secant
- gradient of a tangent
- instantaneous rate of change
- limit
- normal
- product rule
- quotient rule
- secant
- stationary point
- tangent
- turning point
- velocity


###   Notes 


#### Gradients and tangents

A function y=f(x) is differentiable at a point x= a if its graph is
 - continuous, and
 - smooth 
at x=a

The gradient of a secant drawn through 2 points on a curve approximates the gradient of a tangent where accuaracy improves as the distance between the point decreases

$\tan \theta = \text{ the gradient m}$

#### Difference quotients

Average rate of change of f(x) = gradient of chord of a secant $= \dfrac{f(x+h) - f(x)}{h}  $

#### The derivative function and its graph

$\dfrac{dy}{dx} = y' = f'(x) =\lim\limits_{h \to 0} \dfrac{f(x+h) - f(x)}{h}  $

Graphing a derivative funcion f'(x):
 - f'(x) is zero at a stationary point of f(x)
 - f'(x) is positive when f(x) has a positive gradient
 - f'(x) is negative when f(x) has a negative gradient

The derivative at a point represents the instantaneous rate of change


#### Calculating with derivatives

See formulas below<br>

*Average rate of change* of quantity Q with respect to time t = $\dfrac{Q_2-Q_1}{t_2-t_1}$ 
<br><br>
*Instantaneous rate of change* of quantity Q with respect to time t = $\dfrac{dQ}{dt}$ 
<br><br>
*Displacement* measures the distance of an object from a fixed point or origin. Usually positive to the right of the point and negative to the left.
<br><br>
*Velocity* is the instantaneous rate of change of displacement x over time t = $v = \dfrac{dx}{dt}$, for example measured in km/h or $km^{-1}$
<br><br>
*Acceleration* is the instantaneous rate of change of velocity v over time t = $ a = \dfrac{dv}{dt}$, for example measured in km/h/h or $km h^{-2}$


#### Other notes

If two lines with gradients $m_1 \text{ and } m_2$ are perpendicular then $m_1 m_2 = -1$


### Formulas
{{< tabs "tab_547b6871f76d21ce" >}}

{{< tab "Standard view" >}}

<style type="text/css">
#T_standard_cc6ebb3fe6e5f1c6 th.col_heading {
  text-align: left;
  font-size: 1em;
}
#T_standard_cc6ebb3fe6e5f1c6 td {
  text-align: left;
  font-size: 1em;
  padding: 1.5em;
}
</style>
<table id="T_standard_cc6ebb3fe6e5f1c6">
  <thead>
  </thead>
  <tbody>
    <tr>
      <td id="T_standard_cc6ebb3fe6e5f1c6_row0_col0" class="data row0 col0" >$\text{gradient} = m = \dfrac{rise}{run} = \dfrac{y_2-y_1}{x_2-x_1}$</td>
    </tr>
    <tr>
      <td id="T_standard_cc6ebb3fe6e5f1c6_row1_col0" class="data row1 col0" >$ y=f(x)   \,\,\,\,\,\,\,\,\,\,\,\,\,\,\,\,\,\,\,\,\,\,\,\,\,\,\,\,\,\,\,\,\,\,\,\,\,\,\,\,\,\,\,\,\,\,\,\,\,\,   \dfrac{dy}{dx} =\lim\limits_{h \to 0} \dfrac{f(x+h) - f(x)}{h}  $ <br></td>
    </tr>
    <tr>
      <td id="T_standard_cc6ebb3fe6e5f1c6_row2_col0" class="data row2 col0" >$ y=kx   \,\,\,\,\,\,\,\,\,\,\,\,\,\,\,\,\,\,\,\,\,\,\,\,\,\,\,\,\,\,\,\,\,\,\,\,\,\,\,\,\,\,\,\,\,\,\,\,\,\,\,\,\,\,\,   \dfrac{dy}{dx} =k  $ <br></td>
    </tr>
    <tr>
      <td id="T_standard_cc6ebb3fe6e5f1c6_row3_col0" class="data row3 col0" >$ y=k   \,\,\,\,\,\,\,\,\,\,\,\,\,\,\,\,\,\,\,\,\,\,\,\,\,\,\,\,\,\,\,\,\,\,\,\,\,\,\,\,\,\,\,\,\,\,\,\,\,\,\,\,\,\,\,\,\,\,\,   \dfrac{dy}{dx} =0  $ <br></td>
    </tr>
    <tr>
      <td id="T_standard_cc6ebb3fe6e5f1c6_row4_col0" class="data row4 col0" >$ y=x^n   \,\,\,\,\,\,\,\,\,\,\,\,\,\,\,\,\,\,\,\,\,\,\,\,\,\,\,\,\,\,\,\,\,\,\,\,\,\,\,\,\,\,\,\,\,\,\,\,\,\,\,\,\,\,\,\,   \dfrac{dy}{dx} =nx^{n-1}  $ <br></td>
    </tr>
    <tr>
      <td id="T_standard_cc6ebb3fe6e5f1c6_row5_col0" class="data row5 col0" >$ y=kx^n   \,\,\,\,\,\,\,\,\,\,\,\,\,\,\,\,\,\,\,\,\,\,\,\,\,\,\,\,\,\,\,\,\,\,\,\,\,\,\,\,\,\,\,\,\,\,\,\,\,\,\,\,\,   \dfrac{dy}{dx} =knx^{n-1}  $ <br></td>
    </tr>
    <tr>
      <td id="T_standard_cc6ebb3fe6e5f1c6_row6_col0" class="data row6 col0" >$ y=kf(x)   \,\,\,\,\,\,\,\,\,\,\,\,\,\,\,\,\,\,\,\,\,\,\,\,\,\,\,\,\,\,\,\,\,\,\,\,\,\,\,\,\,\,\,\,\,\,\,\,   \dfrac{dy}{dx} =kf'(x)  $ <br></td>
    </tr>
    <tr>
      <td id="T_standard_cc6ebb3fe6e5f1c6_row7_col0" class="data row7 col0" >$ y=f(x) + g(x)   \,\,\,\,\,\,\,\,\,\,\,\,\,\,\,\,\,\,\,\,\,\,\,\,\,\,\,\,\,\,\,\,\,   \dfrac{dy}{dx} =f'(x) + g'(x)  $ <br></td>
    </tr>
    <tr>
      <td id="T_standard_cc6ebb3fe6e5f1c6_row8_col0" class="data row8 col0" >$y=f(x)^n \,\,\,\,\,\,\,\,\,\,\,\,\,\,\,\,\,\,\,\,\,\,\,\,\,\,\,\,\,\,\,\,\,\,\,\,\,\,\,\,\,\,\,\,\,\,\,\,  \dfrac{dy}{dx}=nf'(x)[f(x)]^{n-1}$ <br></td>
    </tr>
    <tr>
      <td id="T_standard_cc6ebb3fe6e5f1c6_row9_col0" class="data row9 col0" >$y=uv \,\,\,\,\,\,\,\,\,\,\,\,\,\,\,\,\,\,\,\,\,\,\,\,\,\,\,\,\,\,\,\,\,\,\,\,\,\,\,\,\,\,\,\,\,\,\,\,\,\,\,\,\,\,\,\,   \dfrac{dy}{dx} = u\dfrac{dv}{dx} + v\dfrac{du}{dx}$ <br></td>
    </tr>
    <tr>
      <td id="T_standard_cc6ebb3fe6e5f1c6_row10_col0" class="data row10 col0" >$y=\dfrac{u}{v} \,\,\,\,\,\,\,\,\,\,\,\,\,\,\,\,\,\,\,\,\,\,\,\,\,\,\,\,\,\,\,\,\,\,\,\,\,\,\,\,\,\,\,\,\,\,\,\,\,\,\,\,\,\,\,\,   \dfrac{dy}{dx} = \dfrac{v\dfrac{du}{dx} - u\dfrac{dv}{dx}}{v^2}$ <br></td>
    </tr>
    <tr>
      <td id="T_standard_cc6ebb3fe6e5f1c6_row11_col0" class="data row11 col0" >$y=g(u) \text { where } u = f(x) \,\,\,\,\,\,\,\,\,\,   \dfrac{dy}{dx} = \dfrac{dy}{du} \times \dfrac{du}{dx} \text { (the chain rule)}$ </td>
    </tr>
  </tbody>
</table>
{{< /tab >}}

{{< tab "Formulas sheet" >}}

<style type="text/css">
#T_formula_sheet_caaed927b5c64ec0 th.col_heading {
  text-align: left;
  font-size: 1em;
}
#T_formula_sheet_caaed927b5c64ec0 td {
  text-align: left;
  font-size: 1em;
  padding: 1.5em;
}
#T_formula_sheet_caaed927b5c64ec0_row0_col0, #T_formula_sheet_caaed927b5c64ec0_row1_col0, #T_formula_sheet_caaed927b5c64ec0_row2_col0, #T_formula_sheet_caaed927b5c64ec0_row3_col0, #T_formula_sheet_caaed927b5c64ec0_row4_col0, #T_formula_sheet_caaed927b5c64ec0_row5_col0, #T_formula_sheet_caaed927b5c64ec0_row6_col0, #T_formula_sheet_caaed927b5c64ec0_row7_col0 {
  background-color: rgba(0,0,0,0);
}
#T_formula_sheet_caaed927b5c64ec0_row8_col0, #T_formula_sheet_caaed927b5c64ec0_row9_col0, #T_formula_sheet_caaed927b5c64ec0_row10_col0, #T_formula_sheet_caaed927b5c64ec0_row11_col0 {
  background-color: rgba(255,194,10, 0.2);
}
</style>
<table id="T_formula_sheet_caaed927b5c64ec0">
  <thead>
  </thead>
  <tbody>
    <tr>
      <td id="T_formula_sheet_caaed927b5c64ec0_row0_col0" class="data row0 col0" >$\text{gradient} = m = \dfrac{rise}{run} = \dfrac{y_2-y_1}{x_2-x_1}$</td>
    </tr>
    <tr>
      <td id="T_formula_sheet_caaed927b5c64ec0_row1_col0" class="data row1 col0" >$ y=f(x)   \,\,\,\,\,\,\,\,\,\,\,\,\,\,\,\,\,\,\,\,\,\,\,\,\,\,\,\,\,\,\,\,\,\,\,\,\,\,\,\,\,\,\,\,\,\,\,\,\,\,   \dfrac{dy}{dx} =\lim\limits_{h \to 0} \dfrac{f(x+h) - f(x)}{h}  $ <br></td>
    </tr>
    <tr>
      <td id="T_formula_sheet_caaed927b5c64ec0_row2_col0" class="data row2 col0" >$ y=kx   \,\,\,\,\,\,\,\,\,\,\,\,\,\,\,\,\,\,\,\,\,\,\,\,\,\,\,\,\,\,\,\,\,\,\,\,\,\,\,\,\,\,\,\,\,\,\,\,\,\,\,\,\,\,\,   \dfrac{dy}{dx} =k  $ <br></td>
    </tr>
    <tr>
      <td id="T_formula_sheet_caaed927b5c64ec0_row3_col0" class="data row3 col0" >$ y=k   \,\,\,\,\,\,\,\,\,\,\,\,\,\,\,\,\,\,\,\,\,\,\,\,\,\,\,\,\,\,\,\,\,\,\,\,\,\,\,\,\,\,\,\,\,\,\,\,\,\,\,\,\,\,\,\,\,\,\,   \dfrac{dy}{dx} =0  $ <br></td>
    </tr>
    <tr>
      <td id="T_formula_sheet_caaed927b5c64ec0_row4_col0" class="data row4 col0" >$ y=x^n   \,\,\,\,\,\,\,\,\,\,\,\,\,\,\,\,\,\,\,\,\,\,\,\,\,\,\,\,\,\,\,\,\,\,\,\,\,\,\,\,\,\,\,\,\,\,\,\,\,\,\,\,\,\,\,\,   \dfrac{dy}{dx} =nx^{n-1}  $ <br></td>
    </tr>
    <tr>
      <td id="T_formula_sheet_caaed927b5c64ec0_row5_col0" class="data row5 col0" >$ y=kx^n   \,\,\,\,\,\,\,\,\,\,\,\,\,\,\,\,\,\,\,\,\,\,\,\,\,\,\,\,\,\,\,\,\,\,\,\,\,\,\,\,\,\,\,\,\,\,\,\,\,\,\,\,\,   \dfrac{dy}{dx} =knx^{n-1}  $ <br></td>
    </tr>
    <tr>
      <td id="T_formula_sheet_caaed927b5c64ec0_row6_col0" class="data row6 col0" >$ y=kf(x)   \,\,\,\,\,\,\,\,\,\,\,\,\,\,\,\,\,\,\,\,\,\,\,\,\,\,\,\,\,\,\,\,\,\,\,\,\,\,\,\,\,\,\,\,\,\,\,\,   \dfrac{dy}{dx} =kf'(x)  $ <br></td>
    </tr>
    <tr>
      <td id="T_formula_sheet_caaed927b5c64ec0_row7_col0" class="data row7 col0" >$ y=f(x) + g(x)   \,\,\,\,\,\,\,\,\,\,\,\,\,\,\,\,\,\,\,\,\,\,\,\,\,\,\,\,\,\,\,\,\,   \dfrac{dy}{dx} =f'(x) + g'(x)  $ <br></td>
    </tr>
    <tr>
      <td id="T_formula_sheet_caaed927b5c64ec0_row8_col0" class="data row8 col0" >$y=f(x)^n \,\,\,\,\,\,\,\,\,\,\,\,\,\,\,\,\,\,\,\,\,\,\,\,\,\,\,\,\,\,\,\,\,\,\,\,\,\,\,\,\,\,\,\,\,\,\,\,  \dfrac{dy}{dx}=nf'(x)[f(x)]^{n-1}$ <br></td>
    </tr>
    <tr>
      <td id="T_formula_sheet_caaed927b5c64ec0_row9_col0" class="data row9 col0" >$y=uv \,\,\,\,\,\,\,\,\,\,\,\,\,\,\,\,\,\,\,\,\,\,\,\,\,\,\,\,\,\,\,\,\,\,\,\,\,\,\,\,\,\,\,\,\,\,\,\,\,\,\,\,\,\,\,\,   \dfrac{dy}{dx} = u\dfrac{dv}{dx} + v\dfrac{du}{dx}$ <br></td>
    </tr>
    <tr>
      <td id="T_formula_sheet_caaed927b5c64ec0_row10_col0" class="data row10 col0" >$y=\dfrac{u}{v} \,\,\,\,\,\,\,\,\,\,\,\,\,\,\,\,\,\,\,\,\,\,\,\,\,\,\,\,\,\,\,\,\,\,\,\,\,\,\,\,\,\,\,\,\,\,\,\,\,\,\,\,\,\,\,\,   \dfrac{dy}{dx} = \dfrac{v\dfrac{du}{dx} - u\dfrac{dv}{dx}}{v^2}$ <br></td>
    </tr>
    <tr>
      <td id="T_formula_sheet_caaed927b5c64ec0_row11_col0" class="data row11 col0" >$y=g(u) \text { where } u = f(x) \,\,\,\,\,\,\,\,\,\,   \dfrac{dy}{dx} = \dfrac{dy}{du} \times \dfrac{du}{dx} \text { (the chain rule)}$ </td>
    </tr>
  </tbody>
</table>
{{< /tab >}}
{{< /tabs >}}
